theories/Codec.v
@@ -1,0 +1,175 @@
+From Coq Require Import ZArith.BinInt.
+From Coq Require Import Lists.List.
+Import ListNotations.
+
+Require Import Utf8.Spec.
+
+(* The definition of UTF-8 prohibits encoding character numbers between *)
+(* U+D800 and U+DFFF and characters bigger than U+10FFFF*)
+Definition utf8_encode_codepoint (n: codepoint) : @option (list byte) :=
+  if (n <? 0) then
+    None
+  else if (n <=? 127) then
+    Some [ n ]
+  else if (n <=? 0x7ff) then
+    let b1 := n / 64 in
+    let b2 := n mod 64 in
+    Some [ 192 + b1; 128 + b2]
+  else if (n <? 0xffff) then
+    let r := n / 64 in
+    let b1 := r / 64 in
+    let b2 := r mod 64 in
+    let b3 := n mod 64 in
+    Some [ 224 + b1; 128 + b2; 128 + b3]
+  else if (n <=? 0x10ffff) then
+    let r1 := n / 64 in
+    let r2 := r1 / 64 in
+    let b1 := r2 / 64 in
+    let b2 := r2 mod 64 in
+    let b3 := r1 mod 64 in
+    let b4 := n mod 64 in
+    Some [ 240 + b1; 128 + b2; 128 + b3; 128 + b4]
+  else
+    None.
+
+Fixpoint utf8_encode (unicode: unicode_str) : (list byte) * (list codepoint) :=
+  match unicode with
+  | [] => ([], [])
+  | code :: unicode_rest =>
+      match utf8_encode_codepoint code with
+      | None => ([], code :: unicode_rest)
+      | Some bytes => 
+          let (bytes_rest, unicode_rest) := utf8_encode unicode_rest in
+          (bytes ++ bytes_rest, unicode_rest)
+      end
+  end.
+
+(* An implementation of the fast and efficient UTF8 decoding DFA *)
+(* presented in the following post: *)
+(* https://bjoern.hoehrmann.de/utf-8/decoder/dfa/ *)
+
+Inductive parsing_state :=
+  Initial
+| Expecting_1_80_BF
+| Expecting_2_80_BF
+| Expecting_3_80_BF
+| Expecting_2_80_9F
+| Expecting_2_A0_BF
+| Expecting_3_90_BF
+| Expecting_3_80_8F.
+
+Inductive byte_range :=
+| Range_00_7F 
+| Range_80_8F
+| Range_90_9F
+| Range_A0_BF
+| Range_C2_DF
+| Byte_E0      
+| Range_E1_EC
+| Byte_ED
+| Range_EE_EF
+| Byte_F0
+| Range_F1_F3
+| Byte_F4
+.
+
+Definition push_bottom_bits (carry: codepoint) (b: byte): codepoint :=
+  carry * 64 + (b mod 64).
+
+Definition extract_7_bits (b: byte) : codepoint :=
+  b mod 128.
+
+Definition extract_5_bits (b: byte) : codepoint :=
+  b mod 32.
+
+Definition extract_4_bits (b: byte) : codepoint :=
+  b mod 16.
+
+Definition extract_3_bits (b: byte) : codepoint :=
+  b mod 8.
+
+Definition byte_range_dec (b: byte) : option byte_range :=
+  if b <? 0 then
+    None
+  else if b <=? 0x7f then
+    Some Range_00_7F
+  else if b <=? 0x8f then
+    Some Range_80_8F
+  else if b <=? 0x9f then
+    Some Range_90_9F
+  else if b <=? 0xbf then
+    Some Range_A0_BF
+  else if b <=? 0xc1 then
+    None
+  else if b <=? 0xdf then
+    Some Range_C2_DF
+  else if b  =? 0xe0 then
+    Some Byte_E0
+  else if b <=? 0xec then
+    Some Range_E1_EC
+  else if b  =? 0xe then
+    Some Byte_ED
+  else if b <=? 0xef then
+    Some Range_EE_EF
+  else if b  =? 0xf0 then
+    Some Byte_F0
+  else if b <=? 0xf3 then
+    Some Range_F1_F3
+  else if b  =? 0xf4 then
+    Some Byte_F4
+  else
+    None.
+
+Inductive parsing_result :=
+  Finished (codep: codepoint)
+| More (state: parsing_state) (acc: codepoint).
+
+Definition next_state (state: parsing_state) (carry: codepoint) (b: byte) : @option parsing_result :=
+  match (state, byte_range_dec b) with
+  | (Initial, Some Range_00_7F) => Some (Finished (extract_7_bits b))
+  | (Initial, Some Range_C2_DF) => Some (More Expecting_1_80_BF (extract_5_bits b))
+  | (Initial, Some Byte_E0)     => Some (More Expecting_2_A0_BF (extract_4_bits b))
+  | (Initial, Some Range_E1_EC)
+  | (Initial, Some Range_EE_EF) => Some (More Expecting_2_80_BF (extract_4_bits b))
+  | (Initial, Some Byte_ED)     => Some (More Expecting_2_80_9F (extract_4_bits b))
+  | (Initial, Some Byte_F0)     => Some (More Expecting_3_90_BF (extract_3_bits b))
+  | (Initial, Some Range_F1_F3) => Some (More Expecting_3_80_BF (extract_3_bits b))
+  | (Initial, Some Byte_F4)     => Some (More Expecting_3_80_8F (extract_3_bits b))
+  | (Initial, _) => None
+  | (Expecting_1_80_BF, Some Range_A0_BF)
+  | (Expecting_1_80_BF, Some Range_90_9F)
+  | (Expecting_1_80_BF, Some Range_80_8F) => Some (Finished (push_bottom_bits carry b))
+  | (Expecting_2_80_BF, Some Range_80_8F)
+  | (Expecting_2_80_BF, Some Range_90_9F)
+  | (Expecting_2_80_9F, Some Range_80_8F)
+  | (Expecting_2_80_9F, Some Range_90_9F)
+  | (Expecting_2_80_BF, Some Range_A0_BF) => Some (More Expecting_1_80_BF (push_bottom_bits carry b))
+  | (Expecting_3_80_BF, Some Range_80_8F)
+  | (Expecting_3_80_BF, Some Range_90_9F)
+  | (Expecting_3_80_BF, Some Range_A0_BF)
+  | (Expecting_3_90_BF, Some Range_90_9F)
+  | (Expecting_3_90_BF, Some Range_A0_BF)
+  | (Expecting_3_80_8F, Some Range_80_8F) => Some (More Expecting_2_80_BF (push_bottom_bits carry b))
+  | (Expecting_2_A0_BF, Some Range_A0_BF) => Some (More Expecting_1_80_BF (push_bottom_bits carry b))
+  | (Expecting_3_80_8F, Some Range_90_9F)
+  | (Expecting_3_80_8F, Some Range_A0_BF) => None
+  | _ => None
+  end.
+
+Fixpoint utf8_dfa_decode_rec (bytes: list byte) (carry: codepoint) (state: parsing_state) (consumed: list byte)
+  : unicode_str * (list byte) :=
+  match bytes with
+  | nil => (nil, nil)
+  | cons b rest =>
+      match next_state state carry b with
+      | Some (Finished codep) =>
+          let (vals, rest) := utf8_dfa_decode_rec rest 0x00 Initial nil in
+          (cons codep vals, rest)
+      | Some (More state codep) =>
+          utf8_dfa_decode_rec rest codep state (b :: consumed)
+      | None => (nil, app consumed bytes)
+      end
+  end.
+
+Definition utf8_dfa_decode (bytes: list byte) : unicode_str * (list byte) :=
+  utf8_dfa_decode_rec bytes 0x00 Initial nil.
